theories/typing/record.v
@@ -8,60 +8,60 @@ From iris.prelude Require Import options.
 (* see product.v, the proof should pretty much the same *)
 Section record.
   Context `{!typeGS Σ}.
-  Lemma split_prod_mt tid ty1 ty2 q l :
+  Lemma split_prod_mt tid ty1 ty2 q l f :
     (l ↦∗{q}: λ vl,
-       ∃ vl1 vl2, ⌜vl = vl1 ++ vl2⌝ ∗ ty1.(ty_own) tid vl1 ∗ ty2.(ty_own) tid vl2)%I
-       ⊣⊢ l ↦∗{q}: ty1.(ty_own) tid ∗ (l +ₗ ty1.(ty_size)) ↦∗{q}: ty2.(ty_own) tid.
+       ∃ v1 v2, ⌜vl = [(f r: v1 :r: v2)%V]⌝ ∗ ty1.(ty_own) tid [v1] ∗ ty2.(ty_own) tid [v2])%I
+       ⊣⊢ (∃ v1, l ↦∗{q} [v1] ∗ ty1.(ty_own) tid [v1]) ∗ (∃ v2, (l +ₗ ty1.(ty_size)) ↦∗{q} [v2] ∗ ty2.(ty_own) tid [v2]).
   Proof.
     iSplit; iIntros "H".
-    - iDestruct "H" as (vl) "[H↦ H]". iDestruct "H" as (vl1 vl2) "(% & H1 & H2)".
-      subst. rewrite heap_mapsto_vec_app. iDestruct "H↦" as "[H↦1 H↦2]".
-      iDestruct (ty_size_eq with "H1") as %->.
-      iSplitL "H1 H↦1"; iExists _; iFrame.
-    - iDestruct "H" as "[H1 H2]". iDestruct "H1" as (vl1) "[H↦1 H1]".
-      iDestruct "H2" as (vl2) "[H↦2 H2]". iExists (vl1 ++ vl2).
-      rewrite heap_mapsto_vec_app. iDestruct (ty_size_eq with "H1") as %->.
+    - iDestruct "H" as (vl) "[H↦ H]". iDestruct "H" as (v1 v2) "(% & H1 & H2)".
+      subst. rewrite heap_mapsto_vec_idemp /= app_nil_r heap_mapsto_vec_app.
+      iDestruct "H↦" as "[H↦1 H↦2]".
+      iDestruct (ty_size_eq with "H1") as %<-.
+      rewrite flattenv_simpl lty_size_singleton -!heap_mapsto_val_idemp.
+      iSplitL "H↦1 H1"; iExists _; iFrame.
+    - iDestruct "H" as "[H1 H2]".
+      iDestruct "H1" as (v1) "[Hvl1 Hown1]".
+      iDestruct "H2" as (v2) "[Hvl2 Hown2]".
+      iExists [(f r: v1 :r: v2)%V].
+      (* so ugly!! *)
+      assert (l ↦∗{q} [(f r: v1 :r: v2)%V] ⊣⊢ l ↦∗{q} ([v1] ++ [v2])).
+      { rewrite heap_mapsto_vec_idemp /= app_nil_r.
+        assert (l ↦∗{q} [v1; v2] ⊣⊢ l ↦∗{q} (flattenv v1 ++ flattenv v2)); first by rewrite heap_mapsto_vec_idemp /= app_nil_r.
+        by rewrite H.
+      }
+      rewrite H heap_mapsto_vec_app. iDestruct (ty_size_eq with "Hown1") as %<-.
       iFrame. iExists _, _. by iFrame.
   Qed.
-  (* FIXME: the RustBelt paper says
-  types in Rust do not just cover a single VALUE:
-  In general, data is laid out in memory
-  and spans multiple locations.
-  However, we have to impose some restrictions
-  on the lists of values accepted by a type:
-  we require that every type has a fixed size [τ].size.
-  This size is used to compute
-  the layout of compound data structures,
-  e.g., for product types.
-  We require that a type only accepts lists whose length matches the size
-  是说，rustbelt的value大小都是1，该怎么办呢！！！
-  不然我会被迫要证明
-    [(l r: v1 :r: v2)%V] = [v1] ++ [v2]
-  而且我们丢失了label的信息
-  *)
+  (* is this even provable? I'm so very not sure *)
+  Lemma val_singleton_vec_exists l q ty tid κ : &{κ}(∃ v, l ↦∗{q} [v] ∗ ty_own ty tid [v]) -∗ &{κ}(l ↦∗{q}: ty_own ty tid).
+  Proof.
+  Admitted.
+
   Program Definition rcons (p : (string * type)) (ty2 : type) : type :=
     let (l, ty1) := p in
     {| ty_size := ty1.(ty_size) + ty2.(ty_size);
-       ty_own tid vl := (∃ vl1 vl2,
-         ⌜vl = vl1 ++ vl2⌝ ∗ ty1.(ty_own) tid vl1 ∗ ty2.(ty_own) tid vl2)%I;
+       ty_own tid vl := (∃ v1 v2, ⌜vl = [(l r: v1 :r: v2)%V]⌝ ∗ ty1.(ty_own) tid [v1] ∗ ty2.(ty_own) tid [v2])%I;
        ty_shr κ tid l :=
          (ty1.(ty_shr) κ tid l ∗
           ty2.(ty_shr) κ tid (l +ₗ ty1.(ty_size)))%I
     |}.
   Next Obligation.
-    iIntros (_ ty2 l ty1 ??) "H".
+    iIntros (_ ty2 f ty1 ??) "H".
     iDestruct "H" as (v1 v2 ->) "[H1 H2]".
-    rewrite app_length. (* without this rewrite, we can't destruct the next equations with -> *)
-    iDestruct (ty_size_eq with "H1") as %->.
-    iDestruct (ty_size_eq with "H2") as %->.
-    done.
+    rewrite /list_ty_size /= Nat.add_0_r.
+    iDestruct (ty_size_eq with "H1") as %<-.
+    iDestruct (ty_size_eq with "H2") as %<-.
+    by rewrite !lty_size_singleton.
   Qed.
   Next Obligation.
-    iIntros (_ ty2 _ ty1 E κ l tid q H) "#Hctx H /= Htok".
+    iIntros (_ ty2 f ty1 E κ l tid q H) "#Hctx H /= Htok".
     rewrite split_prod_mt.
     (* from full borrow we can create a shared reference *)
     (* but first we need to split the full borrow *)
     iMod (bor_sep with "Hctx H") as "(H1 & H2)"; first done.
+    iDestruct (val_singleton_vec_exists with "H1") as "H1".
+    iDestruct (val_singleton_vec_exists with "H2") as "H2".
     (* now we get the sharing predicate from H1 and H2, using ty-share *)
     iMod (ty1.(ty_share) with "Hctx H1 Htok") as "[H1 Htok]"; first apply H.
     iMod (ty2.(ty_share) with "Hctx H2 Htok") as "[H2 Htok]"; first apply H.
@@ -74,8 +74,24 @@ Section record.
     - by iApply (ty1.(ty_shr_mono) with "H⊑").
     - by iApply (ty2.(ty_shr_mono) with "H⊑").
   Qed.
-  (* oh hello, can we hide rcons here it's not really a record *)
-  Definition record := foldr rcons unit0.
+  Program Definition rnil' : type :=
+  {| ty_size := 1;
+     ty_own tid vl := ⌜vl = [rnil%V]⌝%I;
+     ty_shr κ tid l :=
+      emp%I
+  |}.
+  Next Obligation.
+    iIntros (??) "%H". subst vl. iPureIntro. done.
+  Qed.
+  Next Obligation.
+    iIntros (??????) "_ _ Htok". iModIntro. iFrame.
+  Qed.
+  Next Obligation.
+    iIntros (????) "_ //".
+  Qed.
+
+  (* FIXME: because we didn't make val_size rnil to be zero, we can't use unit in foldr (it has size 0), but use our custom 1size rnil type *)
+  Definition record := foldr rcons rnil'.
   Global Instance rcons_proper n l:
   Proper (type_dist2 n ==> type_dist2 n ==> type_dist2 n) (λ t1 t2, rcons (l, t1) t2).
   Proof. solve_type_proper. Qed.
@@ -98,6 +114,7 @@ Section record.
     do 2 rewrite H1.
     apply rcons_proper; first apply H. apply IHForall2.
   Qed.
+
 End record.
 
 Section typing.
@@ -113,6 +130,6 @@ Context `{!typeGS Σ}.
     iIntros (v2) "_ H2".
     iApply wp_value.
     rewrite tctx_interp_singleton tctx_hasty_val.
-    simpl. iExists [v1], [v2]. iFrame. admit.
-  Admitted.
+    simpl. eauto with iFrame.
+  Qed.
 End typing.
