theories/typing/uninit.v
@@ -7,7 +7,7 @@ Section uninit.
   Context `{!typeGS Σ}.
 
   Program Definition uninit_1 : type :=
-    {| st_own tid vl := ⌜length vl = 1%nat⌝%I |}.
+    {| st_own tid vl := ⌜list_ty_size vl = 1%nat⌝%I |}.
   Next Obligation. done. Qed.
 
   Global Instance uninit_1_send : Send uninit_1.
@@ -18,32 +18,64 @@ Section uninit.
 
   Lemma uninit0_sz n : ty_size (uninit0 n) = n.
   Proof. induction n=>//=. by f_equal. Qed.
-
+  Lemma test_ty_own v tid : ⊢ ty_own (uninit0 (val_size v)) tid [v].
+  Proof.
+    iIntros "".
+    iInduction v as [ | | | ] "IH"; simpl.
+    - by iExists [(#l)%V], [].
+    - by iExists [(RecV _ _ _)%V], [].
+    - by iExists [rnil%V], [].
+    - rewrite /uninit0 replicate_add. simpl.
+      (* notice that product accepts a list of values
+      and split the non-flattened list to two parts*)
+      Abort.
+  (*
+    owning an (uninit0 n) already impose restrictions on the elements of vl:
+    each val in vl must be a simple type, that's why the above lemma fails
+  *)
   Lemma uninit0_own n tid vl :
-    ty_own (uninit0 n) tid vl ⊣⊢ ⌜length vl = n⌝.
+    ty_own (uninit0 n) tid vl ⊣⊢ ⌜length vl = n ∧ list_ty_size vl = n⌝.
   Proof.
     iSplit.
     - iIntros "Hvl".
       iInduction n as [|n] "IH" forall (vl); simpl.
       + iDestruct "Hvl" as "%". subst vl. done.
       + iDestruct "Hvl" as (vl1 vl2) "(% & % & Hprod)".
+        assert (length vl1 = 1%nat); first by apply (length1_size1 vl1).
         destruct vl1 as [|v [|]]; try done. subst vl. simpl.
-        iDestruct ("IH" with "Hprod") as "%". iPureIntro. by f_equal.
-    - iIntros "%". subst n. iInduction vl as [|v vl] "IH"; first done.
-      simpl. iExists [v], vl. auto.
+        iDestruct ("IH" with "Hprod") as "[% %]". iPureIntro. 
+        split; [f_equal; apply H | ].
+        by rewrite lty_cons H2 -lty_size_singleton H0.
+    - iIntros "[% %]". subst n. iInduction vl as [|v vl] "IH"; first done.
+      simpl.
+      iExists [v], vl; iSplit; first done. rename H0 into H.
+      destruct v; try (iSplit; first done; iApply "IH";
+        rewrite lty_cons in H; simpl in H;
+        apply eq_add_S in H; iPureIntro; apply H).
+      exfalso. revert H.
+      simpl. rewrite lty_cons. intro H.
+      simpl in H.
+      assert (val_size v1 >= 1%nat) by apply val_gt1.
+      assert (val_size v2 >= 1%nat) by apply val_gt1.
+      assert (list_ty_size vl >= length vl) by apply lty_ge_len.
+      lia.
   Qed.
 
   (* We redefine uninit as an alias of uninit0, so that ty_size and ty_own
      compute directly.  We re-use the sharing from the product as that saves a whole
      lot of work. *)
   Program Definition uninit (n : nat) : type :=
-    {| ty_size := n; ty_own tid vl := ⌜length vl = n⌝%I;
+    {| ty_size := n; ty_own tid vl := ⌜list_ty_size vl = n⌝%I;
        ty_shr := (uninit0 n).(ty_shr) |}.
   Next Obligation. iIntros (???) "%". done. Qed.
   Next Obligation.
     iIntros (n ??????) "LFT Hvl". iApply (ty_share (uninit0 n) with "LFT"); first done.
     iApply (bor_iff with "[] Hvl"). iIntros "!> !>". setoid_rewrite uninit0_own.
-    iSplit; iIntros; done.
+    iSplit; iIntros "H".
+    - iDestruct "H" as (vl) "[? %]". iExists (flatten vl).
+      rewrite heap_mapsto_vec_idemp flatten_size -!flatten_size flatten_idemp !flatten_size.
+      iFrame. done.
+    - iDestruct "H" as (vl) "(Hvl & _ & Hlty)". iExists vl. iFrame.
   Qed.
   Next Obligation. intros. by apply ty_shr_mono. Qed.
 
@@ -55,8 +87,10 @@ Section uninit.
     assert (Copy (uninit0 n)) as [A B].
     { apply product_copy. by apply Forall_replicate, _. }
     split; first by apply _.
-    rewrite uninit0_sz in B. setoid_rewrite uninit0_own in B. done.
-  Qed.
+    rewrite uninit0_sz in B. setoid_rewrite uninit0_own in B.
+    (* let's do some gymnastics! but not now *)
+    admit.
+  Admitted.
 
   Global Instance uninit_send n : Send (uninit n).
   Proof. iIntros (???) "?". done. Qed.
@@ -66,15 +100,18 @@ Section uninit.
 
   (* Unfolding lemma, kep only for backwards compatibility. *)
   Lemma uninit_own n tid vl :
-    (uninit n).(ty_own) tid vl ⊣⊢ ⌜length vl = n⌝.
+    (uninit n).(ty_own) tid vl ⊣⊢ ⌜list_ty_size vl = n⌝.
   Proof. done. Qed.
 
-  Lemma uninit_uninit0_eqtype E L n :
-    eqtype E L (uninit0 n) (uninit n).
+  (* this should be subtype, since uninit n is now stronger than uninit 0 *)
+  Lemma uninit_uninit0_subtype E L n :
+    subtype E L (uninit0 n) (uninit n).
   Proof.
-    apply equiv_eqtype; constructor=>//=.
-    - apply uninit0_sz.
-    - iIntros (??). rewrite uninit0_own. done.
+    apply type_incl_subtype. iIntros "". rewrite /type_incl.
+    iSplit; last iSplit.
+    - by rewrite uninit0_sz /uninit /=.
+    - iIntros "!>" (??) "Hown". rewrite uninit0_own /uninit /=. by iDestruct "Hown" as "[_ ?]".
+    - iIntros "!>" (???) "Hshr". done.
   Qed.
 
   Lemma uninit_product_subtype_cons_r {E L} (n : nat) ty tyl :
@@ -83,20 +120,21 @@ Section uninit.
     subtype E L (uninit (n-ty.(ty_size))) (Π tyl) →
     subtype E L (uninit n) (Π(ty :: tyl)).
   Proof.
-    intros ?%Nat2Z.inj_le. rewrite -!uninit_uninit0_eqtype /uninit0=>Hty Htyl.
-    rewrite -(Nat.sub_add ty.(ty_size) n) // Nat.add_comm // replicate_add
-           -(prod_flatten_r _ _ [_]) /= -prod_app. repeat (done || f_equiv).
-  Qed.
+    intros ?%Nat2Z.inj_le.
+    intros.
+    admit.
+  Admitted.
+
   Lemma uninit_product_subtype_cons_l {E L} (n : nat) ty tyl :
     ty.(ty_size) ≤ n →
     subtype E L ty (uninit ty.(ty_size)) →
     subtype E L (Π tyl) (uninit (n-ty.(ty_size))) →
     subtype E L (Π(ty :: tyl)) (uninit n).
   Proof.
-    intros ?%Nat2Z.inj_le. rewrite -!uninit_uninit0_eqtype /uninit0=>Hty Htyl.
-    rewrite -(Nat.sub_add ty.(ty_size) n) // Nat.add_comm replicate_add
-           -(prod_flatten_r _ _ [_]) /= -prod_app. repeat (done || f_equiv).
-  Qed.
+    intros ?%Nat2Z.inj_le.
+    admit.
+  Admitted.
+
   Lemma uninit_product_eqtype_cons_r {E L} (n : nat) ty tyl :
     ty.(ty_size) ≤ n →
     eqtype E L (uninit ty.(ty_size)) ty →
@@ -117,19 +155,35 @@ Section uninit.
   Lemma uninit_unit_eqtype E L n :
     n = 0%nat →
     eqtype E L (uninit n) unit.
-  Proof. rewrite -uninit_uninit0_eqtype=>->//. Qed.
+  Proof. intros. apply eqtype_unfold. 
+    iIntros (??) "HL !>HE".
+    rewrite /type_equal.
+    iSplit; first done. subst n. rewrite /uninit /unit /=.
+    iSplit; last done.
+    iIntros "!>" (??).
+    iSplit; iIntros "%H"; iPureIntro; last rewrite H lty_size_emp //.
+    destruct vl; try done. exfalso. revert H. rewrite lty_cons.
+    assert (val_size v >= 1%nat) by apply val_gt1. lia.
+  Qed.
   Lemma uninit_unit_eqtype' E L n :
     n = 0%nat →
     eqtype E L unit (uninit n).
-  Proof. rewrite -uninit_uninit0_eqtype=>->//. Qed.
+  Proof. intros. symmetry. rewrite uninit_unit_eqtype; done. Qed.
   Lemma uninit_unit_subtype E L n :
     n = 0%nat →
     subtype E L (uninit n) unit.
-  Proof. rewrite -uninit_uninit0_eqtype=>->//. Qed.
+  Proof. intros. 
+    assert (eqtype E L (uninit n) unit) by rewrite uninit_unit_eqtype //.
+    destruct H0 as [? ?]. apply H0.
+  Qed.
   Lemma uninit_unit_subtype' E L n :
     n = 0%nat →
     subtype E L unit (uninit n).
-  Proof. rewrite -uninit_uninit0_eqtype=>->//. Qed.
+  Proof.
+    intros. 
+    assert (eqtype E L unit (uninit n)) by rewrite uninit_unit_eqtype' //.
+    destruct H0 as [? ?]. apply H0.
+  Qed.
 End uninit.
 
 Global Hint Resolve uninit_product_eqtype_cons_l uninit_product_eqtype_cons_r
